src/lowparse/LowParse_TestLib_SLow_c.c
@@ -1,0 +1,19 @@
+#include "kremlib.h"
+
+#include "Prims.h"
+#include "FStar.h"
+
+#include <stdlib.h>
+#include <stdio.h>
+#include <errno.h>
+#include "LowParse.h"
+#include "LowParse_TestLib_Aux.h"
+
+FStar_Bytes_bytes LowParse_TestLib_SLow_load_file(Prims_string x0)
+{
+    FStar_Bytes_bytes ret;
+    int32_t len;
+    LowParse_TestLib_Aux_load_file(x0, (uint8_t**)&ret.data, &len);
+    ret.length = (uint32_t) len;
+    return ret;
+}
