src/lowparse/LowParse.TestLib.SLow.fst
@@ -1,12 +1,10 @@
-module LowParseTestlib
+module LowParse.TestLib.SLow
 
 open FStar.HyperStack.ST
 open FStar.Bytes
 open FStar.HyperStack.IO
 open FStar.Printf
-open LowParse.Low.Base
 
-module B = FStar.Buffer
 module U32 = FStar.UInt32
 
 #reset-options "--using_facts_from '* -LowParse'"
@@ -17,18 +15,7 @@ module U32 = FStar.UInt32
     there is a fail to parse. *)
 type test_t = (input:FStar.Bytes.bytes) -> Stack (option (FStar.Bytes.bytes * U32.t)) (fun _ -> true) (fun _ _ _ -> true)
 
-(** The type of a unit test.  It takes an input buffer8, parses it,
-    and returns a newly formatted buffer8.  Or it returns None if
-    there is a fail to parse. *)
-type testbuffer_t = (input:buffer8) -> (inputlen:U32.t) -> Stack (option (buffer8 * U32.t)) 
-  (requires(fun h -> is_slice h input inputlen ))
-  (ensures(fun h0 y h1 ->
-    match y with
-    | None -> true
-    | Some (r,o) -> is_slice h1 r o ))
-
 assume val load_file: (filename:string) -> Tot FStar.Bytes.bytes
-assume val load_file_buffer: (filename:string) -> Tot (buffer8 * U32.t)
 
 (** Test one parser+formatter pair against an in-memory buffer of Bytes *)
 let test_bytes (t:test_t) (testname:string) (input:FStar.Bytes.bytes): Stack unit (fun _ -> true) (fun _ _ _ -> true) =
@@ -65,35 +52,4 @@ let test_file (t:test_t) (filename:string): Stack unit (fun _ -> true) (fun _ _ 
   push_frame();
   let input = load_file filename in
   test_bytes t filename input;
-  pop_frame()
-
-(** Test one parser+formatter pair against an in-memory buffer of UInt8.t *)
-let test_buffer (t:testbuffer_t) (testname:string) (input:buffer8) (inputlen:U32.t)
-: Stack unit 
-(requires (fun h -> is_slice h input inputlen))
-(ensures (fun _ _ _ -> true)) =
-  push_frame();
-  print_string (sprintf "==== Testing buffer %s ====\n" testname);
-  let result = t input inputlen in
-  (match result with
-  | Some (formattedresult, offset) -> (
-    if U32.lte offset inputlen then (
-      if B.eqb input formattedresult offset then
-        print_string "Formatted data matches original input data\n"
-      else (
-        print_string "FAIL:  formatted data does not match original input data\n"
-      )
-    ) else (  
-      print_string "Invalid length return - it is longer than the input buffer!"
-    ))
-  | _ -> print_string "Failed to parse\n"
-  ); 
-  print_string (sprintf "==== Finished %s ====\n" testname);
-  pop_frame()
-
-(** Test one parser+formatter pair against a disk file, using buffer *)
-let test_file_buffer (t:testbuffer_t) (filename:string): Stack unit (fun _ -> true) (fun _ _ _ -> true) =
-  push_frame();
-  let input, inputlen = load_file_buffer filename in
-  (*test_buffer t filename input inputlen;*)
   pop_frame()
