src/lowparse/LowParseExample2.fst
@@ -4,6 +4,7 @@ open FStar.HyperStack.ST
 module B32 = FStar.Bytes
 module U32 = FStar.UInt32
 module LP = LowParse.SLow
+module TESTLIB = LowParse.TestLib.SLow
 
 #reset-options "--using_facts_from '* -FStar.Tactics -FStar.Reflection' --z3rlimit 16 --z3cliopt smt.arith.nl=false --max_fuel 2 --max_ifuel 2"
 
